yalla/mell2.v
@@ -30,12 +30,12 @@ Inductive formula :=
 
 Fixpoint dual A :=
 match A with
-| var x     => covar x
-| covar x   => var x
-| tens A B  => parr (dual B) (dual A)
-| parr A B  => tens (dual B) (dual A)
-| oc A      => wn (dual A)
-| wn A      => oc (dual A)
+| var x => covar x
+| covar x => var x
+| tens A B => parr (dual B) (dual A)
+| parr A B => tens (dual B) (dual A)
+| oc A => wn (dual A)
+| wn A => oc (dual A)
 end.
 
 
@@ -43,74 +43,54 @@ end.
 
 Fixpoint mell2ll A :=
 match A with
-| var x    => formulas.var x
-| covar x  => formulas.covar x
+| var x => formulas.var x
+| covar x => formulas.covar x
 | tens A B => formulas.tens (mell2ll A) (mell2ll B)
 | parr A B => formulas.parr (mell2ll A) (mell2ll B)
-| oc A     => formulas.oc (mell2ll A)
-| wn A     => formulas.wn (mell2ll A)
+| oc A => formulas.oc (mell2ll A)
+| wn A => formulas.wn (mell2ll A)
 end.
 
 Lemma mell2ll_inj : injective mell2ll.
 Proof.
 intros A.
-induction A ; intros B Heq ;
-  destruct B ; inversion Heq ;
-  try apply IHA in H0 ;
-  try apply IHA1 in H0 ;
-  try apply IHA2 in H1 ; subst ;
-  reflexivity.
+induction A; intros B Heq; destruct B; inversion Heq ;
+  try apply IHA in H0; try apply IHA1 in H0; try apply IHA2 in H1; subst; reflexivity.
 Qed.
 
 Lemma mell2ll_dual A : formulas.dual (mell2ll A) = mell2ll (dual A).
 Proof. induction A; cbn; rewrite ? IHA, ? IHA1, ? IHA2; reflexivity. Qed.
 
-Lemma mell2ll_map_wn l :
-  map mell2ll (map wn l) = map formulas.wn (map mell2ll l).
+Lemma mell2ll_map_wn l : map mell2ll (map wn l) = map formulas.wn (map mell2ll l).
 Proof. induction l; [ reflexivity | cbn; f_equal; apply IHl ]. Qed.
 
-Lemma mell2ll_map_wn_inv l1 l2 :
-  map formulas.wn l1 = map mell2ll l2 ->
-    { l2' | l2 = map wn l2' /\ l1 = map mell2ll l2' }.
+Lemma mell2ll_map_wn_inv l1 l2 : map formulas.wn l1 = map mell2ll l2 ->
+  { l2' | l2 = map wn l2' & l1 = map mell2ll l2' }.
 Proof.
 induction l1 in l2 |- *; intros Heq; destruct l2 as [|f l2]; inversion Heq.
-- exists nil; split; reflexivity.
+- exists nil; reflexivity.
 - apply IHl1 in H1.
   destruct f; inversion H0; subst.
-  destruct H1 as (l2' & Heq1 & H1); subst.
-  exists (f :: l2'); split; reflexivity.
+  destruct H1 as [l2' -> ->].
+  exists (f :: l2'); reflexivity.
 Qed.
 
 
 (** ** 3. define proofs *)
 
 Inductive mell : list formula -> Type :=
-| ax_r : forall X, mell (covar X :: var X :: nil)
-| ex_r : forall l1 l2, mell l1 ->
-              Permutation_Type l1 l2 -> mell l2
-| mix_r : forall l1 l2, mell l1 -> mell l2 ->
-              mell (l1 ++ l2)
-| tens_r : forall A B l1 l2,
-              mell (A :: l1) -> mell (B :: l2) ->
-              mell (tens A B :: l1 ++ l2)
-| parr_r : forall A B l,
-              mell (A :: B :: l) ->
-              mell (parr A B :: l)
-| oc_r : forall A l,
-              mell (A :: map wn l) ->
-              mell (oc A :: map wn l)
-| de_r : forall A l,
-              mell (A :: l) ->
-              mell (wn A :: l)
-| wk_r : forall A l,
-              mell l ->
-              mell (wn A :: l)
-| co_r : forall A l,
-              mell (wn A :: wn A :: l) ->
-              mell (wn A :: l).
+| ax_r X : mell (covar X :: var X :: nil)
+| ex_r l1 l2 : mell l1 -> Permutation_Type l1 l2 -> mell l2
+| mix_r l1 l2 : mell l1 -> mell l2 -> mell (l1 ++ l2)
+| tens_r A B l1 l2 : mell (A :: l1) -> mell (B :: l2) -> mell (tens A B :: l1 ++ l2)
+| parr_r A B l : mell (A :: B :: l) -> mell (parr A B :: l)
+| oc_r A l : mell (A :: map wn l) -> mell (oc A :: map wn l)
+| de_r A l : mell (A :: l) -> mell (wn A :: l)
+| wk_r A l : mell l -> mell (wn A :: l)
+| co_r A l : mell (wn A :: wn A :: l) -> mell (wn A :: l).
 
 Instance mell_perm : Proper ((@Permutation_Type _) ==> arrow) mell.
-Proof. intros l1 l2 HP pi; apply ex_r with l1; assumption. Qed.
+Proof. intros l1 ? ? ?; apply ex_r with l1; assumption. Qed.
 
 (** ** 4. characterize corresponding [ll] fragment *)
 
@@ -141,43 +121,34 @@ Qed.
 Lemma mellfrag2mell l : ll_def.ll pfrag_mell (map mell2ll l) -> mell l.
 Proof.
 intros pi.
-remember (map mell2ll l) as l0.
+remember (map mell2ll l) as l0 eqn:Heql0.
 revert l Heql0; induction pi using ll_def.ll_nested_ind; intros l' Heql0; subst;
   try now (destruct l'; inversion Heql0; destruct f; inversion H0).
 - symmetry in Heql0; decomp_map_inf Heql0; subst.
   destruct l1; inversion Heql4.
-  destruct x; inversion Heql2.
-  destruct x0; inversion Heql0.
-  subst; subst.
+  destruct x; inversion Heql2; subst.
+  destruct x0; inversion Heql0; subst.
   apply ax_r.
 - cbn in p.
-  apply Permutation_Type_map_inv in p as [l'' Heq HP].
-  apply Permutation_Type_sym in HP.
+  apply Permutation_Type_map_inv in p as [l'' Heq HP%Permutation_Type_sym].
   eapply ex_r, HP.
   apply (IHpi _ Heq).
 - symmetry in Heql0; decomp_map_inf Heql0; subst; symmetry in Heql0.
-  cbn in Heql0; apply mell2ll_map_wn_inv in Heql0 as (l & ? & ?); subst.
-  apply Permutation_Type_map_inv in p as [l' Heq HP]; subst.
-  eapply ex_r;
-    [ apply IHpi; rewrite <- mell2ll_map_wn, <- ? map_app; reflexivity | ].
-  apply Permutation_Type_app_head, Permutation_Type_app_tail.
-  symmetry in HP; apply Permutation_Type_map; assumption.
-- remember (length L) as n.
-  destruct n; inversion eqpmix.
-  destruct n; inversion eqpmix.
-  destruct n; inversion eqpmix.
-  destruct L; inversion Heqn.
-  destruct L; inversion Heqn.
-  destruct L; inversion Heqn.
-  cbn in Heql0.
-  symmetry in Heql0; decomp_map_inf Heql0; subst.
+  cbn in Heql0; apply mell2ll_map_wn_inv in Heql0 as [l -> ->].
+  apply Permutation_Type_map_inv in p as [l' -> HP%Permutation_Type_sym].
+  eapply ex_r; [ apply IHpi; rewrite <- mell2ll_map_wn, <- ? map_app; reflexivity | ].
+  apply Permutation_Type_app_head, Permutation_Type_app_tail, Permutation_Type_map, HP.
+- remember (length L) as n eqn:Heqn.
+  repeat (destruct n; inversion eqpmix).
+  repeat (destruct L; inversion Heqn).
+  cbn in Heql0; symmetry in Heql0; decomp_map_inf Heql0; subst.
   cbn in *; clear H0 H1 H2 H3 Heqn eqpmix.
   destruct l5; inversion Heql4; rewrite app_nil_r; clear Heql4.
   apply mix_r.
   + destruct (In_Forall_inf_in (map mell2ll l2) PL); [ left; reflexivity | ].
-    refine (ll_def.Dependent_Forall_inf_forall_formula _ _ X i _ eq_refl).
+    apply (ll_def.Dependent_Forall_inf_forall_formula _ _ X i _ eq_refl).
   + destruct (In_Forall_inf_in (map mell2ll l4) PL); [ right; left; reflexivity | ].
-    refine (ll_def.Dependent_Forall_inf_forall_formula _ _ X i _ eq_refl).
+    apply (ll_def.Dependent_Forall_inf_forall_formula _ _ X i _ eq_refl).
 - symmetry in Heql0; decomp_map_inf Heql0; subst.
   destruct x; inversion Heql2; subst.
   eapply ex_r; [ apply tens_r | ].
@@ -189,7 +160,7 @@ revert l Heql0; induction pi using ll_def.ll_nested_ind; intros l' Heql0; subst;
   apply parr_r, IHpi; reflexivity.
 - destruct l'; inversion Heql0.
   destruct f; inversion H0; subst.
-  apply mell2ll_map_wn_inv in H1 as (l'' & Heq1 & Heq2); subst.
+  apply mell2ll_map_wn_inv in H1 as [l'' -> ->].
   apply oc_r, IHpi.
   cbn; rewrite mell2ll_map_wn; reflexivity.
 - destruct l'; inversion Heql0.
@@ -219,14 +190,11 @@ Qed.
 
 (** *** cut admissibility *)
 
-Lemma cut_r A l1 l2 :
-  mell (A :: l1) -> mell (dual A :: l2) -> mell (l1 ++ l2).
+Lemma cut_r A l1 l2 : mell (A :: l1) -> mell (dual A :: l2) -> mell (l1 ++ l2).
 Proof.
-intros pi1 pi2.
+intros pi1%mell2mellfrag pi2%mell2mellfrag.
 apply mellfrag2mell.
 rewrite map_app.
-apply mell2mellfrag in pi1.
-apply mell2mellfrag in pi2.
 cbn in pi2; rewrite <- mell2ll_dual in pi2.
 eapply ll_cut.cut_r_axfree; [ | eassumption | eassumption ].
 intros a; destruct a.
